Mostly finish SimpleRecognizerCorrect
But, ugh, we need to propogate back the assumption that the nonterminal
is reachable...

src/Parsers/SimpleRecognizerCorrect.v
@@ -4,6 +4,8 @@ Require Import Fiat.Parsers.ContextFreeGrammar.Core.
 Require Import Fiat.Parsers.StringLike.Core.
 Require Import Fiat.Parsers.SimpleRecognizer Fiat.Parsers.SimpleRecognizerExt.
 Require Import Fiat.Parsers.ContextFreeGrammar.SimpleCorrectness.
+Require Import Fiat.Parsers.ContextFreeGrammar.SimpleCorrectnessMorphisms.
+Require Import Fiat.Common Fiat.Common.Wf.
 
 Section correctness.
   Context {Char} {HSLM : StringLikeMin Char} {HSL : StringLike Char} {HSLP : StringLikeProperties Char} {G : grammar Char}.
@@ -14,9 +16,292 @@ Section correctness.
   (** XXX TODO: remove the above commented out variables if they end up not being necessary. *)
 
   (** To prove the following, look in SimpleRecognizer, SimpleBooleanRecognizerEquality, SimpleRecognizerExt, BooleanRecognizerCorrect, in that order *)
-  Lemma simple_recognizer_correct (str : String) (nt : String.string) t
-    : parse_nonterminal str nt = Some t
-      -> simple_parse_of_correct G str (Lookup G nt) t.
-  Proof.
-  Abort.
+  Context (str : String).
+
+  Local Ltac t'_safe :=
+    idtac;
+    match goal with
+    | _ => assumption
+    | _ => progress destruct_head False
+    | _ => progress simpl in *
+    | _ => progress simpl_simple_parse_of_correct
+    | [ |- context[if ?e then _ else _] ] => destruct e eqn:?
+    | [ H : context[match ?e with _ => _ end] |- _ ] => destruct e eqn:?
+    | _ => intro
+    | _ => congruence
+    | [ H : Some _ = Some _ |- _ ] => inversion H; clear H
+    | [ H : cons _ _ = cons _ _ |- _ ] => inversion H; clear H
+    | [ H : SimpleParseProductionCons _ _ = SimpleParseProductionCons _ _ |- _ ] => inversion H; clear H
+    | _ => progress subst
+    | [ H : context[List.map to_production (nonterminal_to_production (of_nonterminal _))] |- _ ]
+      => rewrite nonterminal_to_production_correct in H
+    | _ => erewrite unsafe_get_correct by eassumption
+    | [ |- is_true (andb _ _) ] => apply Bool.andb_true_iff
+    | [ H : context[substring 0 (length ?str) ?str] |- _ ]
+      => rewrite Properties.substring_correct3' in H
+    | _ => progress unfold option_map in *
+    | [ |- context[length (substring _ 0 _)] ]
+      => rewrite Properties.substring_length
+    | _ => progress rewrite ?Minus.minus_diag, ?Min.min_0_r, ?Min.min_idempotent
+    | [ H : _ |- _ ] => progress rewrite ?Minus.minus_diag, ?Min.min_0_r in H
+    | [ |- context[min ?x ?y - ?y] ] => rewrite <- (NPeano.Nat.sub_min_distr_r x y y)
+    | [ H : EqNat.beq_nat ?x 0 = true |- _ ]
+      => is_var x; apply EqNat.beq_nat_true in H
+    | [ |- cons _ _ = nil ] => exfalso
+    | [ |- _ /\ cons _ _ = nil ] => exfalso
+    | _ => progress specialize_by ltac:(exact eq_refl)
+    | _ => progress specialize_by omega
+    | [ |- ?x = ?x \/ _ ] => left; reflexivity
+    | [ H : context[to_production (production_tl _)] |- _ ]
+      => rewrite production_tl_correct in H
+    | [ H : ?x = cons _ _, H' : appcontext[List.tl ?x] |- _ ]
+      => rewrite H in H'
+    | [ H : cons _ _ = ?x, H' : appcontext[List.tl ?x] |- _ ]
+      => rewrite <- H in H'
+    | [ H : ?x + ?y <= ?z |- _ \/ ?x + min ?a ?y <= ?z ]
+      => right; clear -H; apply Min.min_case_strong; omega
+    | [ H : ?T |- _ \/ ?T ] => right; assumption
+    | [ H : forall x, Some _ = Some x -> _ |- _ ] => specialize (H _ eq_refl)
+    end.
+
+  Local Ltac t'_unsafe :=
+    idtac;
+    match goal with
+    | _ => progress destruct_head or
+    | [ H : andb (EqNat.beq_nat _ 1) (char_at_matches _ _ _) = true |- _ ]
+      => apply Properties.char_at_matches_is_char_no_ex in H; [ | reflexivity || assumption ]
+    | [ H : ?parse_nonterminal (of_nonterminal _) = Some _,
+            IH : forall nt p, ?parse_nonterminal (of_nonterminal nt) = Some p -> _ |- _ ]
+      => specialize (IH _ _ H)
+    | [ |- ?x = ?x /\ _ ] => split; [ reflexivity | ]
+    | [ |- _ /\ ?x = ?x ] => split; [ | reflexivity ]
+    end.
+
+  Local Ltac t' := first [ t'_safe | t'_unsafe ].
+
+  Local Ltac t := repeat t'.
+
+  Section parts.
+    Lemma parse_item'_correct
+          (offset : nat) (len : nat)
+          (Hlen : len = 0 \/ offset + len <= length str)
+          (parse_nonterminal : nonterminal_carrierT -> option simple_parse_of)
+          (parse_nonterminal_correct
+           : forall nt p,
+              parse_nonterminal (of_nonterminal nt) = Some p
+              -> simple_parse_of_item_correct G (substring offset len str) (NonTerminal nt) (SimpleParseNonTerminal nt p))
+          (it : item Char) p
+    : parse_item' str parse_nonterminal offset len it = Some p
+      -> simple_parse_of_item_correct G (substring offset len str) it p.
+    Proof. destruct it, p; t. Qed.
+
+    Section production.
+      Context {len0}
+              (parse_nonterminal
+               : forall (offset : nat) (len : nat),
+                  len <= len0
+                  -> nonterminal_carrierT
+                  -> option simple_parse_of)
+              (parse_nonterminal_correct
+               : forall offset len (Hlen : len = 0 \/ offset + len <= length str) pf nt p,
+                  parse_nonterminal offset len pf (of_nonterminal nt) = Some p
+                  -> simple_parse_of_item_correct G (substring offset len str) (NonTerminal nt) (SimpleParseNonTerminal nt p)).
+
+      Lemma parse_production'_for_correct
+            (splits : production_carrierT -> String -> nat -> nat -> list nat)
+            (offset : nat) (len : nat)
+            (Hlen : len = 0 \/ offset + len <= length str)
+            (pf : len <= len0)
+            (prod_idx : production_carrierT) p
+        : parse_production'_for str parse_nonterminal splits offset pf prod_idx = Some p
+          -> simple_parse_of_production_correct G (substring offset len str) (to_production prod_idx) p.
+      Proof.
+        unfold parse_production'_for.
+        match goal with
+        | [ |- appcontext G[list_rect ?P' ?N' ?C' ?ls'] ]
+          => set (P := P');
+               set (N := N');
+               set (C := C');
+               remember ls' as ls eqn:Hls
+        end;
+          revert offset len Hlen pf.
+        revert prod_idx Hls p.
+        induction ls as [|l ls].
+        { simpl; subst P N C; t. }
+        { destruct p; simpl; unfold C at 1; t;
+          match goal with
+          | [ H : context[List.fold_left _ _ _] |- _ ]
+            => rewrite <- List.fold_left_rev_right, <- List.map_rev in H
+          end;
+          match goal with
+          | [ H : List.fold_right
+                    _ None
+                    (List.map
+                       (fun n => option_SimpleParseProductionCons
+                                   _
+                                   _)
+                       ?ls)
+                  = Some _ |- _ ]
+            => generalize dependent ls; simpl in *;
+               let ls' := fresh in
+               intro ls'; induction ls'
+          end;
+          unfold option_orb, option_SimpleParseProductionCons in *;
+          repeat t'_safe;
+          try solve [ t ];
+          repeat match goal with
+                 | [ H : parse_item' _ _ _ _ _ = Some _ |- _ ]
+                   => apply parse_item'_correct in H;
+                      [
+                      | solve [ t ]..
+                      | intros; eapply parse_nonterminal_correct; [ | eassumption ]; solve [ t ] ]
+                 | [ IH : forall prod_idx pf p offset len Hlen pf',
+                       list_rect ?P ?N ?C ?ls prod_idx offset len pf' = Some p -> _,
+                       H : list_rect ?P ?N ?C ?ls _ _ _ _ = Some _ |- _ ]
+                   => specialize (fun Hlen pf => IH _ pf _ _ _ Hlen _ H)
+                 end;
+          specialize_by ltac:(solve [ t ]);
+          repeat t'_safe.
+          { setoid_rewrite take_take.
+            setoid_rewrite drop_take.
+            setoid_rewrite drop_drop.
+            setoid_rewrite (Plus.plus_comm _ offset).
+            eexists; t; split; eassumption. }
+          { setoid_rewrite take_take.
+            setoid_rewrite drop_take.
+            setoid_rewrite drop_drop.
+            setoid_rewrite (Plus.plus_comm _ offset).
+            eexists; split; [ eassumption | t ]. } }
+      Qed.
+
+      Lemma parse_production'_correct
+            (offset : nat) (len : nat)
+            (Hlen : len = 0 \/ offset + len <= length str)
+            (pf : len <= len0)
+            (prod_idx : production_carrierT) p
+        : parse_production' str parse_nonterminal offset pf prod_idx = Some p
+          -> simple_parse_of_production_correct G (substring offset len str) (to_production prod_idx) p.
+      Proof.
+        apply parse_production'_for_correct; assumption.
+      Qed.
+    End production.
+
+    Section productions.
+      Context {len0}
+              (parse_nonterminal
+               : forall (offset : nat)
+                        (len : nat)
+                        (pf : len <= len0),
+                  nonterminal_carrierT -> option simple_parse_of)
+              (parse_nonterminal_correct
+               : forall offset len (Hlen : len = 0 \/ offset + len <= length str) pf nt p,
+                  parse_nonterminal offset len pf (of_nonterminal nt) = Some p
+                  -> simple_parse_of_item_correct G (substring offset len str) (NonTerminal nt) (SimpleParseNonTerminal nt p)).
+
+      Definition parse_productions'_correct
+                 (offset : nat) (len : nat)
+                 (Hlen : len = 0 \/ offset + len <= length str)
+                 (pf : len <= len0)
+                 (prods : list production_carrierT)
+                 p
+        : parse_productions' str parse_nonterminal offset pf prods = Some p
+          -> simple_parse_of_correct G (substring offset len str) (List.map to_production prods) p.
+      Proof.
+        unfold parse_productions'.
+        revert p; induction prods as [|x xs IHxs]; intros; destruct p; unfold option_simple_parse_of_orb in *;
+          t.
+        { eapply parse_production'_correct; [ eassumption | t.. | eassumption ]. }
+        { eapply parse_production'_correct; [ eassumption | t.. | eassumption ]. }
+      Qed.
+    End productions.
+
+    Section nonterminals.
+      Section step.
+        Context {len0 valid_len}
+                (parse_nonterminal
+                 : forall (p : nat * nat),
+                    prod_relation lt lt p (len0, valid_len)
+                    -> forall (valid : nonterminals_listT)
+                              (offset : nat) (len : nat),
+                      len <= fst p -> nonterminal_carrierT -> option simple_parse_of)
+                (parse_nonterminal_correct
+                 : forall p0 wf valid offset len (Hlen : len = 0 \/ offset + len <= length str) pf nt p,
+                    parse_nonterminal p0 wf valid offset len pf (of_nonterminal nt) = Some p
+                    -> simple_parse_of_item_correct G (substring offset len str) (NonTerminal nt) (SimpleParseNonTerminal nt p)).
+
+        Lemma parse_nonterminal_step_correct
+                   (valid : nonterminals_listT)
+                   (offset : nat) (len : nat)
+                   (Hlen : len = 0 \/ offset + len <= length str)
+                   (pf : len <= len0)
+                   nt
+                   p
+          : parse_nonterminal_step str parse_nonterminal valid offset pf (of_nonterminal nt) = Some p
+            -> simple_parse_of_correct G (substring offset len str) (List.map to_production (nonterminal_to_production (of_nonterminal nt))) p.
+        Proof.
+          specialize (fun p00 p01 wf valid => @parse_nonterminal_correct (p00, p01) wf valid).
+          unfold parse_nonterminal_step, option_rect; t;
+            unfold sumbool_rect in *; t;
+              let H := match goal with H : parse_productions' _ _ _ _ _ = Some _ |- _ => H end in
+              (eapply parse_productions'_correct in H;
+               [ assumption | .. ]);
+                eauto with nocore;
+                omega.
+        Qed.
+      End step.
+
+      Section wf.
+        Lemma parse_nonterminal_or_abort_correct
+        : forall (p : nat * nat)
+                 (valid : nonterminals_listT)
+                 (offset : nat) (len : nat)
+                 (Hlen : len = 0 \/ offset + len <= length str)
+                 (pf : len <= fst p)
+                 nt
+                 pt,
+          parse_nonterminal_or_abort str p valid offset pf (of_nonterminal nt) = Some pt
+          -> simple_parse_of_correct G (substring offset len str) (List.map to_production (nonterminal_to_production (of_nonterminal nt))) pt.
+        Proof.
+          unfold parse_nonterminal_or_abort.
+          intro p.
+          let Rwf := match goal with |- appcontext[Fix ?Rwf] => Rwf end in
+          induction (Rwf p) as [?? IH].
+          intros ??????? HF.
+          rewrite Fix5_eq in HF
+                          by (intros; apply parse_nonterminal_step_ext; assumption).
+          eapply parse_nonterminal_step_correct; [ | assumption | eassumption ].
+          simpl; intros; simpl_simple_parse_of_correct.
+        Admitted.
+        (*
+        Lemma parse_nonterminal'_correct
+              (nt : nonterminal_carrierT)
+          : option simple_parse_of
+            := @parse_nonterminal_or_abort
+                 (length str, nonterminals_length initial_nonterminals_data)
+                 initial_nonterminals_data
+                 0 (length str)
+                 (le_n _) nt.
+
+          Definition parse_nonterminal
+                     (nt : String.string)
+          : option simple_parse_of
+            := parse_nonterminal' (of_nonterminal nt).*)
+      End wf.
+    End nonterminals.
+(*
+    Definition parse_item
+               (it : item Char)
+      : option simple_parse_of_item
+      := parse_item' parse_nonterminal' 0 (length str) it.
+
+    Definition parse_production
+               (pat : production_carrierT)
+      : option simple_parse_of_production
+      := parse_production' (parse_nonterminal_or_abort (length str, nonterminals_length initial_nonterminals_data) initial_nonterminals_data) 0 (reflexivity _) pat.
+
+    Definition parse_productions
+               (pats : list production_carrierT)
+      : option simple_parse_of
+      := parse_productions' (parse_nonterminal_or_abort (length str, nonterminals_length initial_nonterminals_data) initial_nonterminals_data) 0 (reflexivity _) pats. *)
+  End parts.
 End correctness.
